src/imp/lifting.v
@@ -1,12 +1,50 @@
-(* wp for implang, using a customed notion of wp *)
+(* wp for implang *)
+From iris.algebra.lib Require Import excl_auth.
 From iris.base_logic Require Import gen_heap.
+From iris.program_logic Require Import weakestpre adequacy.
 From iris_imp_lang Require Import lifting_expr.
 From iris_imp_lang.imp Require Import notation.
+From RecordUpdate Require Import RecordSet.
+Import RecordSetNotations.
+
+Definition to_val s := match s with skip => Some tt | _ => None end.
+
+Lemma implang_mixin F : LanguageMixin(observation := Empty_set) (λ _, skip) to_val
+    (λ s σ obs s' σ' es, obs = [] ∧ es = [] ∧ step F s σ s' σ').
+Proof.
+  split.
+  - by intros [].
+  - by destruct e; inversion 1.
+  - by intros ?????? (? & ? & H); inv H.
+Qed.
+
+Lemma eval_expr_det e r m v1 : eval_expr e r m v1 → forall v2, eval_expr e r m v2 →
+  v1 = v2.
+Proof.
+  induction 1; inversion 1; subst; try congruence.
+  - specialize (IHeval_expr1 _ ltac:(eassumption)).
+    specialize (IHeval_expr2 _ ltac:(eassumption)); congruence.
+  - specialize (IHeval_expr _ ltac:(eassumption)); congruence.
+Qed.
+
+Ltac expr_det := match goal with H1 : eval_expr' ?a ?b ?v1, H2 : eval_expr' ?a ?b ?v2 |- _ =>
+  let H := fresh "Heq" in pose proof (eval_expr_det _ _ _ _ H1 _ H2) as H; clear H2; inv H end.
+
+Class impGS hlc Σ :=
+  { impGS_gen_heapGS :: gen_heapGS loc val Σ;
+    impGS_envGS :: envGS val Σ;
+    impGS_invGS :: invGS_gen hlc Σ;
+    impGS_stackGS :: inG Σ (excl_authR nat);
+    impGS_stack_gname : gname
+  }.
 
 Section wp.
 
-Context `{!gen_heapGS loc val Σ} `{!envGS val Σ} `{!invGS_gen HasNoLc Σ}.
+Context `{!impGS hlc Σ}.
 Variable (F : func_env).
+Notation γ := impGS_stack_gname.
+
+Canonical Structure imp_lang := Language (implang_mixin F).
 
 Implicit Types (ρ : @env_state val) (σ : gmap loc val).
 
@@ -18,144 +56,152 @@ Fixpoint make_stack (k : stack) : env_state * nat :=
 
 Definition stack_depth k := snd (make_stack k).
 
-Definition stack_match ρ r k := let '(ρ0, n) := make_stack k in (stack_level n ∗ ⌜ρ = <[n := r]>ρ0⌝)%I.
+Definition state_ctx (s : state) := (gen_heap_interp s.(m) ∗
+  let '(ρ0, n) := make_stack s.(k) in
+    env_auth (<[n := s.(ρ)]>ρ0) ∗ own γ (●E n))%I.
 
-Lemma stack_env_match ρ r k : stack_match ρ r k ⊢ env_match ρ r.
-Proof.
-  unfold stack_match.
-  destruct (make_stack k) eqn: Hk.
-  unfold stack_level; split => ?; monPred.unseal.
-  iIntros "(<- & ->)"; iPureIntro.
-  by rewrite lookup_insert.
-Qed.
+Global Instance implang_irisG : irisGS_gen hlc imp_lang Σ := {
+  iris_invGS := _;
+  state_interp s _ _ _ := state_ctx s;
+  fork_post _ := True%I;
+  num_laters_per_step _ := 0%nat;
+  state_interp_mono _ _ _ _ := fupd_intro _ _;
+}.
 
-Definition wp_pre (wp : coPset -d> stmt -d> assert -d> assert) :
-    coPset -d> stmt -d> assert -d> assert := λ E s Q,
-  ((⌜s = skip⌝ ∧ |={E}=> Q) ∨
-   (∀ σ ρ, ⎡state_interp σ ρ⎤ ={E,∅}=∗ ∀ r k, stack_match ρ r k -∗
-    ∃ s' r' σ' k',
-        ⌜step F s (Build_state r σ k) s' (Build_state r' σ' k')⌝ ∗
-        ▷ |={∅,E}=> ∃ ρ', ⎡state_interp σ' ρ' ∗ (stack_match ρ' r' k' ∗ wp E s' Q) (stack_depth k')⎤))%I.
+Definition stack_top n := (⎡own γ (◯E n)⎤ ∗ stack_level n)%I.
 
-Local Instance wp_contractive : Contractive (wp_pre).
-Proof.
-  rewrite /wp_pre /= => n wp wp' Hwp E s Q.
-  do 29 (f_contractive || f_equiv). apply Hwp.
-Qed.
-
-Local Definition wp_def := fixpoint wp_pre.
-Local Definition wp_aux : seal (@wp_def). Proof. by eexists. Qed.
-Definition wp := wp_aux.(unseal).
-Local Lemma wp_unseal   : wp = @wp_def.
-Proof. rewrite -wp_aux.(seal_eq) //. Qed.
-
-Lemma wp_unfold E s Q : wp E s Q ⊣⊢ wp_pre wp E s Q.
-Proof. rewrite wp_unseal. apply (fixpoint_unfold wp_pre). Qed.
+Definition wp E s (Q : assert) : assert := (∀ n, stack_top n -∗
+  ⎡wp NotStuck E s (λ _, ∃ n', own γ (◯E n') ∗ Q n')⎤)%I.
 
 Lemma wp_mono E s P Q : <obj> (P -∗ Q) ⊢ wp E s P -∗ wp E s Q.
 Proof.
-  split => n; monPred.unseal.
-  iIntros "HPQ" (? <-) "H".
-  iLöb as "IH" forall (n s P Q).
-  rewrite !wp_unfold /wp_pre; monPred.unseal.
-  iDestruct "H" as "[(% & H) | H]".
-  - iLeft; iSplit => //.
-    by iApply "HPQ".
-  - iRight.
-    iIntros (???<-) "S"; iMod ("H" with "[//] S") as "H".
-    iIntros "!> %%%<- Hstack".
-    rewrite {1 3}/stack_match.
-    destruct (make_stack _) eqn: Hstack.
-    rewrite /stack_level; monPred.unseal.
-    iDestruct "Hstack" as %(<- & ?).
-    iDestruct ("H" with "[//] []") as (?????) "H".
-    { setoid_rewrite Hstack; done. }
-    iExists _, _, _, _; iSplit => //.
-    iNext; iMod "H" as (?) "($ & $ & H)".
-    iApply ("IH" with "[HPQ] H").
-    iIntros (??); iApply "HPQ".
+  iIntros "HPQ H" (?) "N".
+  iSpecialize ("H" with "N").
+  iApply (wp_wand with "H").
+  iIntros (_) "(% & $ & ?)".
+  iStopProof; split => ?; monPred.unseal.
+  iIntros "(HPQ & H)"; by iApply "HPQ".
 Qed.
 
 Lemma wp_skip E R : R ⊢ wp E skip R.
 Proof.
-  iIntros "R".
-  rewrite wp_unfold /wp_pre. iLeft.
-  iSplit; done.
+  iIntros "R" (?) "(N & L)".
+  rewrite /wp wp_unfold /wp_pre /=.
+  rewrite embed_fupd; iModIntro; iFrame.
+  by iApply (stack_level_embed with "L").
 Qed.
 
-Lemma var_e : forall x v σ ρ r k,
-  stack_match ρ r k ∗ x ↦v v ∗ ⎡state_interp σ ρ⎤ ⊢ ⌜r !! x = Some v⌝.
+Lemma var_e : forall n x v s,
+  stack_top n ∗ x ↦v v ∗ ⎡state_ctx s⎤ ⊢ ⌜s.(ρ) !! x = Some v⌝.
 Proof.
-  intros; rewrite /stack_match /stack_level;
-  destruct (make_stack k) eqn: Hk.
+  intros; rewrite /state_ctx /stack_top /stack_level.
+  destruct (make_stack _) eqn: Hk.
   split => ?; monPred.unseal.
-  iIntros "((-> & ->) & Hx & (_ & Hρ))".
+  iIntros "((N & <-) & Hx & _ & Hρ & N')".
+  iCombine "N N'" gives %->%excl_auth_agree_L.
   iDestruct (var_e with "[$Hx $Hρ]") as %?.
   by rewrite /env_to_environ lookup_insert in H.
 Qed.
 
-Lemma var_update : forall x v v' σ ρ r k,
-  stack_match ρ r k ∗ x ↦v v ∗ ⎡state_interp σ ρ⎤ ⊢
-  |==> ∃ ρ', stack_match ρ' (<[x := v']>r) k ∗ x ↦v v' ∗ ⎡state_interp σ ρ'⎤.
+Lemma var_update : forall n x v v' s,
+  stack_top n ∗ x ↦v v ∗ ⎡state_ctx s⎤ ⊢
+  |==> stack_top n ∗ x ↦v v' ∗ ⎡state_ctx (s <| ρ ::= <[x := v']> |>)⎤.
 Proof.
-  intros; rewrite /stack_match /stack_level;
-  destruct (make_stack k) eqn: Hk.
+  intros; rewrite /state_ctx /stack_top /stack_level.
+  destruct (make_stack _) eqn: Hk.
   split => ?; monPred.unseal.
-  iIntros "((-> & ->) & Hx & ($ & Hρ))".
-  iMod (var_update with "[$Hx $Hρ]") as "($ & $)".
-  iModIntro; iSplit; try done.
-  rewrite /set_var lookup_insert insert_insert H //.
+  iIntros "((N & %H) & Hx & $ & Hρ & N')"; hnf in H; subst.
+  iCombine "N N'" gives %<-%excl_auth_agree_L.
+  iMod (var_update with "[$Hx $Hρ]") as "(? & $)".
+  rewrite /set_var lookup_insert insert_insert; by iFrame.
 Qed.
 
-Lemma stack_match_stack_depth ρ r k (P : assert) i:
-  (stack_match ρ r k) i -∗ P i -∗
-  (stack_match ρ r k ∗ P) (stack_depth k).
+Lemma state_level_elim s n : state_ctx s -∗ own γ (◯E n) -∗ ⌜n = stack_depth s.(k)⌝.
 Proof.
-  unfold stack_match, stack_depth.
-  destruct (make_stack k).
-  rewrite /stack_level; monPred.unseal.
-  iIntros "(<- & ->) $". done.
-Qed.
-
-Lemma stack_match_embed ρ r k (P : assert) : stack_match ρ r k -∗ P -∗
-  ⎡(stack_match ρ r k ∗ P) (stack_depth k)⎤.
-Proof.
-  unfold stack_match, stack_depth.
-  destruct (make_stack k).
-  iIntros "(#? & %) P"; iApply stack_level_embed; by iFrame "# ∗".
+  rewrite /state_ctx /stack_depth.
+  destruct (make_stack _).
+  iIntros "(_ & _ & Ha) Hb".
+  by iCombine "Ha Hb" gives %->%excl_auth_agree_L.
 Qed.
 
 Lemma wp_seq E s1 s2 Q : wp E s1 (▷ wp E s2 Q) ⊢ wp E (Sseq s1 s2) Q.
 Proof.
-  split => n.
-  iIntros "H".
-  iLöb as "IH" forall (s1 s2 Q n).
-  rewrite wp_unfold [wp _ (s1;;s2)%S _]wp_unfold /wp_pre.
-  monPred.unseal.
-  iRight.
-  iIntros (???<-) "S".
-  iDestruct "H" as "[[-> >Hs1] | H]".
-  - iApply fupd_mask_intro; first set_solver; iIntros "Hclose" (???<-) "Hstack".
-    iExists _, _, _, _. iSplit.
-    { iPureIntro. apply SeqS2. }
-    { iNext; iFrame.
-      rewrite /stack_match /stack_depth.
-      destruct (make_stack x2).
-      rewrite /stack_level; monPred.unseal.
-      iDestruct "Hstack" as (<-) "$".
-      iMod "Hclose". iModIntro; iSplit => //.
-    }
-  - iDestruct ("H" with "[//] [$]") as ">H".
-    iModIntro.
-    iIntros (r k ? <-) "Hmatch".
-    iDestruct ("H" with "[//] [$Hmatch]") as (????) "(% & H)".
-    iExists _, _, _, _.
-    iSplit; first by (iPureIntro; econstructor).
-    clear.
-    iNext; iMod "H" as (ρ) "($ & ? & ?)"; iModIntro.
-    rewrite -monPred_at_sep.
-    iApply (stack_match_stack_depth with "[$] [-]").
-    iApply "IH"; iFrame.
+  split => n; rewrite /wp /stack_top /stack_level; monPred.unseal.
+  iIntros "H" (?? <-) "(N & ->)".
+  iSpecialize ("H" with "[//] [$N //]").
+  clear.
+  iLöb as "IH" forall (s1 s2 Q).
+  rewrite wp_unfold (wp_unfold _ _ (s1;; s2)%S) /wp_pre /=.
+  iIntros (?????) "S".
+  destruct (to_val s1) eqn: Hs1.
+  - destruct s1; inv Hs1.
+    iMod "H" as (?) "(N & H)".
+    iApply fupd_mask_intro; first set_solver; iIntros "Hclose".
+    iSplit.
+    { iPureIntro. eexists _, _, _, _; split; first done; split; first done.
+      apply SeqS2. }
+    iIntros (??? (-> & -> & H)); inv H.
+    { inv H6. }
+    iDestruct (state_level_elim with "S N") as %->; iFrame.
+    iIntros "_ !> !> !>".
+    iMod "Hclose".
+    iModIntro; iSplit => //.
+    by iApply ("H" with "[//] [$N //]").
+  - iDestruct ("H" $! _ O [] [] O with "[$]") as ">(%Hred & H)".
+    iModIntro; iSplit.
+    { iPureIntro; destruct Hred as (? & ? & ? & ? & -> & -> & H).
+      eexists _, _, _, _; split; first done; split; first done.
+      by constructor. }
+    iIntros (??? (-> & -> & H)) "?".
+    inv H.
+    iMod ("H" with "[//] [$]") as "H".
+    iIntros "!> !> !>".
+    iMod "H"; iMod "H" as "($ & H & $)".
+    by iApply "IH".
+Qed.
+
+Lemma wp_expr_app E e Q n s : wp_expr E e Q -∗ stack_top n -∗
+  ⎡state_ctx s⎤ ={E}=∗ ∃ v, ⌜eval_expr e s.(ρ) s.(m) v⌝ ∗ stack_top n ∗
+  ⎡state_ctx s⎤ ∗ Q v.
+Proof.
+  rewrite /state_ctx; wp_expr.unseal.
+  iIntros "H (N & #L) (Hσ & Hρ)".
+  destruct (make_stack _) eqn: Hstack; iDestruct "Hρ" as "(Hρ & N')".
+  iMod ("H" with "[$Hσ $Hρ]") as (?) "(He & ($ & $) & HQ)".
+  iCombine "N N'" gives %->%excl_auth_agree_L.
+  iFrame; iFrame "#".
+  iStopProof; split => ?; rewrite /stack_level; monPred.unseal; rewrite monPred_at_intuitionistically.
+  iIntros "(% & H)"; iApply ("H" with "[//]").
+  by rewrite lookup_insert.
+Qed.
+
+Lemma stack_top_embed n (P : assert) : stack_top n -∗ P -∗ ⎡own γ (◯E n) ∗ P n⎤.
+Proof.
+  iIntros "($ & #L) P". by iApply stack_level_embed.
+Qed.
+
+Lemma wp_assign E x e Q : wp_expr E e (λ v, (∃ v0, x ↦v v0) ∗
+  ▷ (x ↦v v -∗ Q)) ⊢ wp E (Sassign x e) Q.
+Proof.
+  iIntros "H" (?) "N".
+  rewrite /wp wp_unfold /wp_pre /=.
+  iIntros (?????) "S".
+  iMod (wp_expr_app with "H N S") as (? He) "(N & S & (% & Hx) & Hpost)".
+  rewrite embed_fupd.
+  iApply fupd_mask_intro; first set_solver; iIntros "Hclose"; iSplit.
+  { iPureIntro; eexists _, _, _, _; split; first done; split; first done; by constructor. }
+  iIntros (??? (-> & -> & H)) "?".
+  inv H.
+  eapply eval_expr_det in He; last done; subst.
+  rewrite embed_fupd; iModIntro; iNext.
+  rewrite embed_fupd; iModIntro.
+  iDestruct (var_e with "[$Hx $S $N]") as %?.
+  iMod (var_update with "[$Hx $S $N]") as "(N & ? & $)".
+  iMod "Hclose".
+  rewrite /= bi.sep_emp wp_unfold /wp_pre /=.
+  do 2 (rewrite embed_fupd; iModIntro).
+  iPoseProof (stack_top_embed with "N [-]") as "($ & H)"; last done.
+  by iApply "Hpost".
 Qed.
 
 Definition get_params f := let 'Func params _ _ _ := f in params.
@@ -177,16 +223,13 @@ Definition call_assert E f vs x R := (⇑ (stack_retainer f -∗ stackframe f vs
     (∃ vs, ⌜stack_size f = length vs⌝ ∧ stackframe f vs) ∗
     ⇓ ((∃ v, points_to_var x v) ∗ ▷ (points_to_var x v -∗ R))))))%I.
 
-Lemma wp_exprs_app E es Q σ ρ : wp_exprs E es Q -∗ ⎡state_interp σ ρ⎤ ={E}=∗
-  ∃ vs, (∀ r k, env_match ρ r -∗ ⌜eval_exprs' es (Build_state r σ k) vs⌝) ∗ ⎡state_interp σ ρ⎤ ∗ Q vs.
+Lemma wp_exprs_app E es Q n s : wp_exprs E es Q -∗ stack_top n -∗ ⎡state_ctx s⎤ ={E}=∗
+  ∃ vs, ⌜eval_exprs' es s vs⌝ ∗ stack_top n ∗ ⎡state_ctx s⎤ ∗ Q vs.
 Proof.
-  iIntros "Hes S"; iInduction es as [|e es] "IH" forall (Q); simpl.
-  - iFrame. iIntros "!> %% ?"; iPureIntro; constructor.
-  - wp_expr.unseal.
-    iMod ("Hes" with "S") as (?) "(He & S & Hes)".
-    iMod ("IH" with "Hes S") as (?) "(Hes & $ & $)".
-    iIntros "!> %% Henv".
-    iDestruct ("He" with "Henv") as %?; iDestruct ("Hes" $! _ k with "Henv") as %?.
+  iIntros "Hes N S"; iInduction es as [|e es] "IH" forall (Q); simpl.
+  - iFrame. iPureIntro; constructor.
+  - iMod (wp_expr_app with "Hes N S") as (??) "(N & S & Hes)".
+    iMod ("IH" with "Hes N S") as (??) "$".
     iPureIntro; by constructor.
 Qed.
 
@@ -199,22 +242,24 @@ Proof.
     eapply IHk; eauto; lia.
 Qed.
 
-Lemma add_frame σ ρ r k xs vs : ⎡state_interp σ ρ⎤ ∗ stack_match ρ r k ⊢
-  |==> ∃ ρ', ⎡state_interp σ ρ'⎤ ∗ ⇑ (stack_match ρ' (bind_vars xs vs) (r :: k) ∗
+Lemma add_frame s n xs vs : ⎡state_ctx s⎤ ∗ stack_top n ⊢
+  |==> ⎡state_ctx (s <| ρ := bind_vars xs vs |> <| k:= s.(ρ) :: s.(k) |>)⎤ ∗ ⇑ (stack_top (S n) ∗
     assert_of (λ n, stack_frag n (/ pos_to_Qp (Pos.of_nat (1 + size (bind_vars xs vs))))%Qp 1%Qp (bind_vars xs vs))).
 Proof.
-  intros; rewrite /stack_match /=.
-  destruct (make_stack k) eqn: Hk.
-  iIntros "(Hρ & #Hl & ->)".
-  iMod (state_interp_alloc_frame _ _ (S n) with "Hρ") as "($ & ?)".
+  intros; rewrite /state_ctx /stack_top /=.
+  iIntros "((Hσ & Hρ) & N & #L)".
+  destruct (make_stack _) eqn: Hstack; iDestruct "Hρ" as "(Hρ & N')".
+  iCombine "N N'" gives %->%excl_auth_agree_L.
+  iMod (state_interp_alloc_frame _ _ (S n) with "[$Hσ $Hρ]") as "(($ & $) & ?)".
   { rewrite lookup_insert_ne //.
     eapply stack_depth_max; eauto. }
+  iMod (own_update_2 with "N' N") as "($ & N)".
+  { apply excl_auth_update. }
   iModIntro.
-  rewrite -!up1_sep.
-  iPoseProof (stack_level_up with "Hl") as "$".
-  rewrite -up1_objective; iSplit; first done.
+  rewrite -!up1_sep -up1_objective; iFrame.
+  iSplit; first by iApply stack_level_up.
   iStopProof; split => ?; rewrite /stack_level; monPred.unseal; rewrite monPred_at_intuitionistically /=.
-  iIntros "((<- & _) & $)".
+  iIntros "(<- & $)".
 Qed.
 
 Lemma pure_sep_equiv P (Q R : iProp Σ) : (P → (Q ⊣⊢ R)) → ⌜P⌝ ∗ Q ⊣⊢ ⌜P⌝ ∗ R.
@@ -261,20 +306,37 @@ Proof.
       rewrite length_zip_with_l_eq //.
 Qed.
 
-Lemma remove_frame σ ρ r r0 k q r' : ⎡state_interp σ ρ⎤ ∗ stack_match ρ r (r0 :: k) ∗ assert_of (λ n, stack_frag n q 1%Qp r') ⊢
-  |==> ∃ ρ', ⎡state_interp σ ρ'⎤ ∗ ⇓ stack_match ρ' r0 k.
+Lemma remove_frame s r0 k0 n q r' : s.(k) = r0 :: k0 →
+  ⎡state_ctx s⎤ ∗ stack_top (S n) ∗ assert_of (λ n, stack_frag n q 1%Qp r') ⊢
+  |==> ⎡state_ctx (s <| ρ := r0 |> <| k := k0 |>)⎤ ∗ ⇓ stack_top n.
 Proof.
-  intros; rewrite /stack_match /=.
-  destruct (make_stack k) eqn: Hk.
-  iIntros "(Hρ & (#Hl & ->) & H)".
-  iMod (state_interp_dealloc_frame _ _ (S n) with "[$Hρ H]") as "$".
+  intros; rewrite /state_ctx /stack_top H /=.
+  destruct (make_stack _) eqn: Hk.
+  iIntros "((Hσ & Hρ & N') & (N & #Hl) & H)".
+  iCombine "N N'" gives %[=]%excl_auth_agree_L; subst.
+  iMod (state_interp_dealloc_frame _ _ (S n) with "[$Hσ $Hρ H]") as "($ & ?)".
   { iApply (stack_level_embed with "Hl H"). }
+  iMod (own_update_2 with "N' N") as "($ & N)".
+  { apply excl_auth_update. }
   iModIntro.
-  rewrite -!down1_sep.
+  rewrite -!down1_sep -down1_objective; iFrame.
   iPoseProof (stack_level_down with "Hl") as "$".
-  rewrite -down1_objective; iPureIntro.
-  apply (delete_insert _ _ r).
+  iClear "#"; iStopProof; do 2 f_equiv.
+  apply (delete_insert _ _ s.(ρ)).
   rewrite lookup_insert_ne //; eapply stack_depth_max; eauto.
+Qed.
+
+Lemma eval_exprs_det e s v1 : eval_exprs' e s v1 → forall v2, eval_exprs' e s v2 →
+  v1 = v2.
+Proof.
+  induction 1; inversion 1; subst; try congruence.
+  expr_det; f_equiv; auto.
+Qed.
+
+Lemma bi_entails_obj (P Q : assert) : (P ⊢ Q) → ⊢ <obj> (P -∗ Q).
+Proof.
+  intros; split => n; monPred.unseal.
+  iIntros "_" (???); by iApply monPred_in_entails.
 Qed.
 
 Lemma wp_call E x f es Q : wp_exprs E es (λ vs, ∃ fd, ⌜F !! f = Some fd ∧
@@ -282,301 +344,200 @@ Lemma wp_call E x f es Q : wp_exprs E es (λ vs, ∃ fd, ⌜F !! f = Some fd ∧
   ▷ call_assert E fd (vs ++ repeat (NumV 0) (length (get_locals fd))) x Q) ⊢
   wp E (Scall x f es) Q.
 Proof.
-  iIntros "H".
-  rewrite wp_unfold /wp_pre; iRight.
-  iIntros (??) "S".
-  iMod (wp_exprs_app with "H S") as (?) "(Hes & S & %fd & (% & %Hlen & %) & H)".
+  iIntros "H" (?) "N".
+  rewrite wp_unfold /wp_pre /=.
+  iIntros (?????) "S".
+  iMod (wp_exprs_app with "H N S") as (? Hes) "(N & S & %fd & (%Hf & %Hlen & %Hnodup) & H)".
   destruct fd; simpl in *.
-  iApply fupd_mask_intro; first set_solver; iIntros "Hclose" (??) "Hstack".
-  iDestruct ("Hes" with "[Hstack]") as %?; first by iApply stack_env_match.
-  iExists _, _, _, _; iSplit.
-  { iPureIntro; by econstructor. }
-  iNext.
-  iMod (add_frame with "[$S $Hstack]") as (?) "($ & Hstack)".
-  iMod "Hclose" as "_"; iModIntro; simpl.
+  rewrite embed_fupd; iApply fupd_mask_intro; first set_solver; iIntros "Hclose"; iSplit.
+  { iPureIntro. eexists _, _, _, _; split; first done; split; first done; by constructor. }
+  iIntros (??? (-> & -> & H)) "?"; inv H.
+  eapply eval_exprs_det in Hes; last done; subst.
+  rewrite embed_fupd; iModIntro; iNext; rewrite embed_fupd; iModIntro.
+  iMod (add_frame with "[$S $N]") as "($ & N)".
+  rewrite embed_fupd; iMod "Hclose" as "_"; iModIntro; simpl.
   iApply up1_obj_elim; iApply up1_mono; last first.
   { rewrite /call_assert.
-    iCombine "H Hstack" as "H"; rewrite !up1_sep; iApply "H". }
-  iIntros "(H & Hstack & Hframe)".
-  iAssert (stack_level (S (stack_depth k))) with "[Hstack]" as "#Hl".
+    iCombine "H N" as "H"; rewrite !up1_sep; iApply "H". }
+  iIntros "(H & (N & #L) & Hframe)".
+  (*iAssert (stack_level (S (stack_depth k))) with "[Hstack]" as "#Hl".
   { rewrite /stack_match /stack_depth /=. destruct (make_stack k); iDestruct "Hstack" as "($ & _)". }
-  iApply (stack_match_embed with "Hstack").
+  iApply (stack_match_embed with "Hstack").*)
   assert (length (func_params ++ func_locals) = length (vs ++ repeat (NumV 0) (length func_locals))).
   { rewrite !app_length repeat_length; f_equal.
     rewrite -Hlen; by eapply Forall2_length. }
   iPoseProof (bi.equiv_entails_1_1 with "[Hframe]") as "Hframe"; first by apply split_stackframe.
   { iFrame; eauto. }
   iDestruct "Hframe" as "(Hret & Hframe)".
-  iApply wp_seq. iApply wp_mono; last by iApply ("H" with "Hret Hframe").
-  rewrite monPred_objectively_unfold; iIntros "!>" (?); monPred.unseal.
-  iIntros (??) "H !>".
-  rewrite wp_unfold /wp_pre; wp_expr.unseal; monPred.unseal.
-  iRight; iStopProof; do 8 f_equiv.
-  iIntros ">(% & He & (Hσ & Hρ) & Hret & Hframe & (% & Hx) & H)".
+  rewrite bi.sep_emp; iApply (wp_seq with "[-N] [$N //]").
+  iApply wp_mono; last by iApply ("H" with "Hret Hframe").
+  iApply bi_entails_obj.
+  iIntros "H !>" (?) "N".
+  rewrite wp_unfold /wp_pre /=.
+  iIntros (?????) "S".
+  iMod (wp_expr_app with "H N S") as (? He) "(N & S & Hret & Hframe & H)".
+  iStopProof; split => ?; monPred.unseal.
+  iIntros "(N & (Hσ & Hρ) & Hret & Hframe & (% & Hx) & H)".
+  destruct (make_stack _) eqn: Hk; iDestruct "Hρ" as "(Hρ & N')".
   iDestruct (stack_ra.var_e with "[$Hx $Hρ]") as %?.
-  iApply fupd_mask_intro; first set_solver; iIntros "Hclose" (???<-) "Hstack".
-  rewrite {1}/stack_match.
-  destruct (make_stack _) eqn: Hstack.
-  rewrite /stack_level; monPred.unseal.
-  iDestruct "Hstack" as %([=] & ->).
+  rewrite /stack_top /stack_level; monPred.unseal.
+  iDestruct "N" as "(N & ->)".
   rewrite /stack_retainer /stack_level; monPred.unseal.
   iDestruct "Hret" as (? [=]) "Hret"; subst; simpl in *.
-  iDestruct ("He" with "[//] []") as %?.
-  { by rewrite lookup_insert. }
-  destruct x3; try done.
-  iExists _,_, _, _; iSplit.
-  { iPureIntro; by econstructor. }
-  iNext.
+  iCombine "N N'" gives %->%excl_auth_agree_L.
+  destruct σ0; simpl in *; destruct k; try done.
+  iApply fupd_mask_intro; first set_solver; iIntros "Hclose"; iSplit.
+  { iPureIntro. eexists _, _, _, _; split; first done; split; first done; by econstructor. }
+  iIntros (??? (-> & -> & Hstep)) "?"; inv Hstep; simpl in *.
+  eapply eval_expr_det in He; last done; subst.
+  iIntros "!> !> !>".
   iDestruct "Hframe" as (??) "Hframe".
-  iPoseProof (monPred_in_entails with "[Hσ Hρ Hret Hframe]") as "H'"; first apply remove_frame.
+  iPoseProof (monPred_in_entails with "[Hσ Hρ N N' Hret Hframe]") as "H'"; first apply (remove_frame (Build_state ρ0 m0 (ρ1 :: k0))).
+  { done. }
   { monPred.unseal; iFrame.
-    iAssert (stack_retainer (Func func_params func_locals func_body func_ret) (S x4)) with "[Hret]" as "Hret".
+    iAssert (stack_retainer (Func func_params func_locals func_body func_ret) (S x1)) with "[Hret]" as "Hret".
     { rewrite /stack_retainer /stack_level; monPred.unseal; by iFrame. }
     iCombine "Hret Hframe" as "H".
     rewrite -monPred_at_sep monPred_in_equiv; last by symmetry; apply split_stackframe; rewrite ?app_length.
     monPred.unseal; iDestruct "H" as (?) "(_ & $)".
-    rewrite /stack_match /stack_level; setoid_rewrite Hstack; by monPred.unseal. }
-  monPred.unseal; iMod "H'" as (?) "(S & Hstack)".
+    rewrite Hk; iFrame.
+    rewrite /stack_top /stack_level; monPred.unseal; by iFrame. }
+  monPred.unseal; iMod "H'" as "(S & Hstack)".
   iPoseProof (monPred_in_entails with "[S Hstack Hx]") as "H'"; first apply var_update.
   { monPred.unseal; iFrame. }
-  monPred.unseal; iMod "H'" as (?) "(Hstack & Hx & $)".
+  monPred.unseal; iMod "H'" as "(Hstack & Hx & $)".
   iMod "Hclose"; iModIntro.
-  iSplitR "H Hx".
-  - rewrite /stack_match /stack_depth; destruct (make_stack x3); monPred.unseal.
-    iDestruct "Hstack" as "(_ & $)"; rewrite /stack_level; by monPred.unseal.
-  - simpl in Hstack.
-    rewrite /stack_depth; destruct (make_stack _).
-    inv Hstack.
-    rewrite -wp_skip; by iApply "H".
-Qed.
-
-Lemma wp_assign E x e Q : wp_expr E e (λ v, (∃ v0, x ↦v v0) ∗
-  ▷ (x ↦v v -∗ Q)) ⊢ wp E (Sassign x e) Q.
-Proof.
-  iIntros "H".
-  rewrite wp_unfold /wp_pre /stack_depth. iRight.
-  iIntros (??) "S".
-  wp_expr.unseal.
-  iMod ("H" with "S") as (?) "(He & S & (% & Hx) & Hpost)".
-  iApply fupd_mask_intro; first set_solver; iIntros "Hclose" (r k) "Hstack".
-  iDestruct (var_e with "[$Hx $S $Hstack]") as %?.
-  iDestruct ("He" with "[Hstack]") as %?; first by iApply stack_env_match.
-  iExists _, _, _, _; iSplit.
-  { iPureIntro; by constructor. }
-  iNext.
-  iMod (var_update with "[$Hx $S $Hstack]") as (?) "(match & ? & $)".
-  iMod "Hclose"; iModIntro.
-  simpl.
-  iApply (stack_match_embed with "[$]").
-  rewrite -wp_skip. by iApply "Hpost".
+  rewrite bi.sep_emp wp_unfold /wp_pre /=.
+  rewrite /stack_top; monPred.unseal; iDestruct "Hstack" as "($ & ?)".
+  by iApply "H".
 Qed.
 
 Lemma wp_alloc E x Q : (∃ v0, x ↦v v0) ∗
   ▷ (∀ l, points_to_var x (LocV l) -∗ l ↦ NumV 0 -∗ Q) ⊢ wp E (Salloc x) Q.
 Proof.
-  iIntros "H".
-  rewrite wp_unfold /wp_pre. iRight.
-  iIntros (??) "S".
+  iIntros "H" (?) "N".
+  rewrite wp_unfold /wp_pre /=.
+  iIntros (?????) "S".
   iDestruct "H" as "((% & Hx) & Hpost)".
-  iApply fupd_mask_intro; first set_solver; iIntros "Hclose" (??) "Hstack".
-  iDestruct (var_e with "[$Hx $S $Hstack]") as %?.
-  iExists _, _, _, _; iSplit.
-  { iPureIntro; by econstructor. }
-  iNext.
-  iMod (var_update with "[$Hx $S $Hstack]") as (?) "(? & Hx & S)".
-  iMod (state_interp_alloc with "S") as "($ & S)".
-  { apply next_loc_new. }
-  iMod "Hclose"; iModIntro.
-  iApply (stack_match_embed with "[$]").
-  rewrite -wp_skip. by iApply ("Hpost" with "[$]").
+  rewrite embed_fupd; iApply fupd_mask_intro; first set_solver; iIntros "Hclose".
+  iDestruct (var_e with "[$Hx $S $N]") as %He.
+  iSplit.
+  { iPureIntro. eexists _, _, _, _; split; first done; split; first done; apply alloc_fresh. }
+  iIntros (??? (-> & -> & H)) "?"; inv H.
+  rewrite embed_fupd; iModIntro; iNext; rewrite embed_fupd; iModIntro.
+  iMod (var_update with "[$Hx $S $N]") as "(N & Hx & S)".
+  rewrite /state_ctx.
+  destruct (make_stack _) eqn: Hk.
+  iDestruct "S" as "(Hσ & Hρ & $)".
+  iMod (state_interp_alloc with "[$Hσ $Hρ]") as "($ & S)"; first done.
+  iMod "Hclose".
+  rewrite wp_unfold /wp_pre /= bi.sep_emp.
+  do 2 (rewrite embed_fupd; iModIntro); iExists _; iApply (stack_top_embed with "N").
+  by iApply ("Hpost" with "Hx").
 Qed.
 
 Lemma wp_store E e1 e2 Q : wp_expr E e2 (λ v, wp_expr E e1 (λ v1, ∃ l v0, ⌜v1 = LocV l⌝ ∧
   l ↦ v0 ∗ ▷ (l ↦ v -∗ Q))) ⊢ wp E (Sstore e1 e2) Q.
 Proof.
-  iIntros "H".
-  rewrite wp_unfold /wp_pre. iRight.
-  iIntros (??) "S".
-  wp_expr.unseal.
-  iMod ("H" with "S") as (?) "(He2 & S & H)".
-  wp_expr.unseal.
-  iMod ("H" with "S") as (?) "(He1 & S & % & % & -> & Hl & Hpost)".
-  iApply fupd_mask_intro; first set_solver; iIntros "Hclose" (??) "Hstack".
-  iDestruct (state_interp_load with "S Hl") as %?.
-  iDestruct ("He1" with "[Hstack]") as %?; first by iApply stack_env_match.
-  iDestruct ("He2" with "[Hstack]") as %?; first by iApply stack_env_match.
-  iExists _, _, _, _; iSplit.
-  { iPureIntro; by econstructor. }
-  iNext.
-  iMod (state_interp_store with "S Hl") as "($ & ?)"; iFrame.
-  iMod "Hclose"; iModIntro.
-  iApply (stack_match_embed with "[$]").
-  rewrite -wp_skip. by iApply "Hpost".
+  iIntros "H" (?) "N".
+  rewrite wp_unfold /wp_pre /=.
+  iIntros (?????) "S".
+  iMod (wp_expr_app with "H N S") as (? He2) "(N & S & H)".
+  iMod (wp_expr_app with "H N S") as (? He1) "(N & S & % & % & -> & Hl & Hpost)".
+  rewrite embed_fupd; iApply fupd_mask_intro; first set_solver; iIntros "Hclose".
+  rewrite /state_ctx.
+  destruct (make_stack _) eqn: Hk; iDestruct "S" as "(Hσ & Hρ & N')".
+  iDestruct (state_interp_load with "[$Hσ $Hρ] Hl") as %Hl.
+  iSplit.
+  { iPureIntro. eexists _, _, _, _; split; first done; split; first done; by econstructor. }
+  iIntros (??? (-> & -> & H)) "?"; inv H.
+  eapply eval_expr_det in He2; last done.
+  eapply eval_expr_det in He1; last done; inv He1.
+  rewrite embed_fupd; iModIntro; iNext; rewrite embed_fupd; iModIntro.
+  rewrite /= Hk.
+  iMod (state_interp_store with "[$Hσ $Hρ] Hl") as "(($ & ?) & ?)"; iFrame.
+  iMod "Hclose".
+  rewrite wp_unfold /wp_pre /= bi.sep_emp.
+  do 2 (rewrite embed_fupd; iModIntro); iExists _; iApply (stack_top_embed with "N").
+  by iApply "Hpost".
 Qed.
 
 Lemma wp_if E e s1 s2 Q : wp_expr E e (λ v, ∃ n, ⌜v = NumV n⌝ ∧
   ▷ wp E (if Z.eqb n 0 then s2 else s1) Q) ⊢ wp E (Sif e s1 s2) Q.
 Proof.
-  iIntros "H".
-  rewrite wp_unfold /wp_pre. iRight.
-  iIntros (??) "S".
-  wp_expr.unseal.
-  iMod ("H" with "S") as (?) "(He & S & % & -> & H)".
-  iApply fupd_mask_intro; first set_solver; iIntros "Hclose" (??) "Hstack".
-  iDestruct ("He" with "[Hstack]") as %?; first by iApply stack_env_match.
-  iExists _, _, _, _; iSplit.
-  { iPureIntro; by econstructor. }
-  iNext; iFrame.
-  iApply (stack_match_embed with "[$]").
-  iMod "Hclose". iApply "H".
+  iIntros "H" (?) "N".
+  rewrite wp_unfold /wp_pre /=.
+  iIntros (?????) "S".
+  iMod (wp_expr_app with "H N S") as (? He) "(N & S & % & -> & H)".
+  rewrite embed_fupd; iApply fupd_mask_intro; first set_solver; iIntros "Hclose"; iSplit.
+  { iPureIntro. eexists _, _, _, _; split; first done; split; first done; by econstructor. }
+  iIntros (??? (-> & -> & H)) "?"; inv H.
+  eapply eval_expr_det in He; last done; inv He.
+  rewrite embed_fupd; iModIntro; iNext; rewrite embed_fupd; iModIntro; iFrame.
+  rewrite bi.sep_emp.
+  iMod "Hclose". rewrite embed_fupd; iModIntro. iApply ("H" with "N").
 Qed.
 
 Lemma wp_while E e s Q : wp_expr E e (λ v, ∃ n, ⌜v = NumV n⌝ ∧
   ▷ if Z.eqb n 0 then Q else wp E s (▷ wp E (Swhile e s) Q)) ⊢
   wp E (Swhile e s) Q.
 Proof.
-  iIntros "H".
-  rewrite {2}[wp _ (Swhile _ _) _]wp_unfold /wp_pre. iRight.
-  iIntros (??) "S".
-  wp_expr.unseal.
-  iMod ("H" with "S") as (?) "(He & S & % & -> & H)".
-  iApply fupd_mask_intro; first set_solver; iIntros "Hclose" (??) "Hstack".
-  iDestruct ("He" with "[Hstack]") as %?; first by iApply stack_env_match.
-  destruct (Z.eqb n 0) eqn:?.
-  -  iExists _, _, _, _; iSplit.
-    { iPureIntro. econstructor; eauto. }
-    iNext; iFrame.
-    iMod "Hclose" as "_"; iModIntro.
-    rewrite Heqb -wp_skip //.
-    by iApply (stack_match_embed with "[$]").
-  - iExists _, _, _, _; iSplit.
-    { iPureIntro; econstructor; eauto. }
-    iNext; iFrame.
-    iMod "Hclose" as "_"; iModIntro.
-    rewrite Heqb -wp_seq //.
-    by iApply (stack_match_embed with "[$]").
+  iIntros "H" (l) "N".
+  rewrite wp_unfold /wp_pre /=.
+  iIntros (?????) "S".
+  iMod (wp_expr_app with "H N S") as (? He) "(N & S & % & -> & H)".
+  rewrite embed_fupd; iApply fupd_mask_intro; first set_solver; iIntros "Hclose".
+  destruct (Z.eqb n 0) eqn:Hn.
+  - iSplit.
+    { iPureIntro. eexists _, _, _, _; split; first done; split; first done; by constructor. }
+    iIntros (??? (-> & -> & H)) "?"; inv H.
+    eapply eval_expr_det in He; last done; inv He.
+    rewrite Hn; iFrame.
+    rewrite embed_fupd; iModIntro; iNext; rewrite embed_fupd; iModIntro; iFrame.
+    rewrite wp_unfold /wp_pre /= bi.sep_emp.
+    iMod "Hclose". do 2 (rewrite embed_fupd; iModIntro).
+    iExists _; by iApply (stack_top_embed with "N").
+  - iSplit.
+    { iPureIntro. eexists _, _, _, _; split; first done; split; first done; by constructor. }
+    iIntros (??? (-> & -> & H)) "?"; inv H.
+    eapply eval_expr_det in He; last done; inv He.
+    rewrite Hn; iFrame.
+    rewrite embed_fupd; iModIntro; iNext; rewrite embed_fupd; iModIntro; iFrame.
+    iMod "Hclose". rewrite embed_fupd; iModIntro.
+    rewrite bi.sep_emp.
+    by iApply (wp_seq with "H").
 Qed.
 
 End wp.
 
 Section adequacy.
 
-(* generalize? *)
-Definition not_stuck F s σ := s = skip ∨
-  (∃ s' σ', step F s σ s' σ').
+Class impGpreS Σ :=
+  { impGpreS_gen_heapGS :: gen_heapGpreS loc val Σ;
+    impGpreS_envGpreS :: inG Σ (@envR val);
+    impGpreS_invGpreS :: invGpreS Σ;
+    impGpreS_stackGpreS :: inG Σ (excl_authR nat)
+  }.
 
-Record adequate F s (σ1 : state) (φ : state → Prop) := {
-  adequate_result σ2 :
-   step_star F s σ1 skip σ2 → φ σ2;
-  adequate_not_stuck s2 σ2 :
-   step_star F s σ1 s2 σ2 →
-   not_stuck F s2 σ2
-}.
-
-Lemma adequate_alt F s1 σ1 (φ : state → Prop) :
-  adequate F s1 σ1 φ ↔ ∀ s2 σ2,
-    step_star F s1 σ1 s2 σ2 →
-      (s2 = skip → φ σ2) ∧
-      (not_stuck F s2 σ2).
+Lemma wp_adequacy hlc Σ `{!impGpreS Σ} F (s : stmt) σ φ :
+  (∀ `{!impGS hlc Σ}, ⊢ |={⊤}=> wp F ⊤ s (⌜φ⌝)) →
+  adequate(Λ := imp_lang F) NotStuck s (Build_state ∅ σ []) (λ _ _, φ).
 Proof.
-  split.
-  - intros []; naive_solver.
-  - constructor; naive_solver.
-Qed.
-
-Inductive nsteps (F : func_env) : nat → stmt → state → stmt → state → Prop :=
-  | nsteps_refl s σ :
-     nsteps F 0 s σ s σ
-  | nsteps_l n s1 σ1 s2 σ2 s3 σ3 :
-     step F s1 σ1 s2 σ2 →
-     nsteps F n s2 σ2 s3 σ3 →
-     nsteps F (S n) s1 σ1 s3 σ3.
-Local Hint Constructors nsteps : core.
-
-Lemma step_star_nsteps F s1 σ1 s2 σ2 :
-  step_star F s1 σ1 s2 σ2 ↔ ∃ n, nsteps F n s1 σ1 s2 σ2.
-Proof.
-  split.
-  - induction 1; firstorder eauto.
-  - intros (n & Hsteps).
-    induction Hsteps; eauto using Step0, Step1.
-Qed.
-
-Lemma eval_expr_det e r m v1 : eval_expr e r m v1 → forall v2, eval_expr e r m v2 →
-  v1 = v2.
-Proof.
-  induction 1; inversion 1; subst; try congruence.
-  - specialize (IHeval_expr1 _ ltac:(eassumption)).
-    specialize (IHeval_expr2 _ ltac:(eassumption)); congruence.
-  - specialize (IHeval_expr _ ltac:(eassumption)); congruence.
-Qed.
-
-Ltac expr_det := match goal with H1 : eval_expr' ?a ?b ?v1, H2 : eval_expr' ?a ?b ?v2 |- _ =>
-  let H := fresh "Heq" in pose proof (eval_expr_det _ _ _ _ H1 _ H2) as H; clear H2; inv H end.
-
-Lemma eval_exprs_det e σ v1 : eval_exprs' e σ v1 → forall v2, eval_exprs' e σ v2 →
-  v1 = v2.
-Proof.
-  induction 1; inversion 1; subst; try congruence.
-  expr_det; f_equiv; auto.
-Qed.
-
-Lemma step_det F s σ s1 σ1 s2 σ2 : step F s σ s1 σ1 → step F s σ s2 σ2 →
-  s1 = s2 ∧ σ1 = σ2.
-Proof.
-  intros; generalize dependent s2.
-  induction H; inversion 1; subst; repeat expr_det; try done; try congruence.
-  - edestruct IHstep; first done; by subst.
-  - inv H.
-  - inv H6.
-  - rewrite H in H7; inv H7. eapply eval_exprs_det in H1; last done. by subst.
-Qed.
-
-Lemma wp_adequacy Σ `{!gen_heapGpreS loc val Σ} `{!inG Σ (@envR val)} `{!invGpreS Σ} F s σ φ :
-  (∀ `{!gen_heapGS loc val Σ} `{!envGS val Σ} `{Hinv : !invGS_gen HasNoLc Σ},
-     ⊢ |={⊤}=> wp F ⊤ s (⌜φ⌝)) →
-  adequate F s (Build_state ∅ σ []) (λ _, φ).
-Proof.
-  intros Hwp. apply adequate_alt; intros s2 σ2 H.
-  eapply uPred.pure_soundness.
-  apply step_star_nsteps in H as (n & H).
-  eapply (step_fupdN_soundness_gen _ HasNoLc n n).
-  iIntros (Hinv) "_".
+  intros; eapply (wp_adequacy_gen hlc); first apply _.
+  intros; iIntros.
   iMod (gen_heap_init σ) as (?) "[Hh _]".
   iMod (env_init ∅) as (?) "(He & _)".
-  iPoseProof (monPred_in_entails _ _ (Hwp _ _ _) O with "[]") as "Hwp"; clear Hwp.
-  { by monPred.unseal. }
-  rewrite monPred_at_fupd; iMod "Hwp".
-  iAssert (stack_match {[0 := ∅]} ∅ [] O) as "-#Hstack".
-  { rewrite /stack_match /stack_level; by monPred.unseal. }
-
-  set (r := ∅) in *; clearbody r.
-  set (k := []) in *; clearbody k.
-  set (ρ := {[0 := r]}); clearbody ρ.
-  set (l := 0); clearbody l.
-  iInduction n as [|n] "IH" forall (σ ρ r k l s H).
-  - inv H.
-     rewrite wp_unfold /wp_pre; monPred.unseal.
-    iDestruct "Hwp" as "[Hwp | Hwp]".
-    + iDestruct "Hwp" as "(-> & >%)".
-      iApply fupd_mask_intro; first set_solver.
-      iIntros "_"; iPureIntro; rewrite /not_stuck /=; auto.
-    + iMod ("Hwp" with "[//] [$Hh $He]") as "Hwp".
-      iDestruct ("Hwp" with "[//] Hstack") as (???? Hstep) "H".
-      iPureIntro; split.
-      * intros ->; inv Hstep.
-      * right; eauto.
-  - inv H.
-    rewrite wp_unfold /wp_pre; monPred.unseal; iDestruct "Hwp" as "[Hwp | Hwp]".
-    { iDestruct "Hwp" as "(-> & _)"; inv H3. }
-    iMod ("Hwp" with "[//] [$Hh $He]") as "Hwp".
-    iDestruct ("Hwp" with "[//] Hstack") as (???? Hstep) "H".
-    eapply step_det in H3; last done.
-    destruct H3 as (<- & <-).
-    iModIntro; simpl.
-    iModIntro; iNext.
-    iMod "H" as (?) "((Hh & He) & Hstack & H)".
-    iApply ("IH" with "[//] Hh He H Hstack").
+  iMod (own_alloc) as (?) "H"; first apply (excl_auth_valid O); iDestruct "H" as "(? & N)".
+  set HI := Build_impGS _ _ _ _ _ _ γ.
+  iExists (λ σ _, state_ctx σ), (λ _, True%I).
+  rewrite /state_ctx /=; iFrame.
+  iPoseProof (monPred_in_entails _ _ (H _) O with "[]") as "Hwp"; clear H;
+    monPred.unseal; first done.
+  iMod "Hwp" as "Hwp".
+  rewrite /wp /stack_top /stack_level; monPred.unseal.
+  iSpecialize ("Hwp" with "[//] [$N //]").
+  iApply (wp_wand with "Hwp").
+  iIntros "!> % (% & _ & $)".
 Qed.
 
 End adequacy.
